linux/pkvm/proofs/early_alloc/generated_spec.v
@@ -16,17 +16,20 @@ Section spec.
   Notation PAGE := (PAGES 1).
 
   (* Definition of type [region]. *)
-  Definition region_rec : (loc * nat * nat -d> typeO) → (loc * nat * nat -d> typeO) := (λ self patt__,
+  Definition region_rec : (loc * Z * Z -d> typeO) → (loc * Z * Z -d> typeO) := (λ self patt__,
     let base := patt__.1.1 in
     let given := patt__.1.2 in
     let remaining := patt__.2 in
     let z_cur : Z := (base.2 + given * PAGE_SIZE)%Z in
     let z_end : Z := (base.2 + (given + remaining) * PAGE_SIZE)%Z in
-    struct struct_region [@{type}
-      (own_constrained (nonshr_constraint ((base.1, z_cur) ◁ₗ uninit (PAGES remaining))) (value (void*) (base))) ;
+    constrained (struct struct_region [@{type}
+      (own_constrained (nonshr_constraint ((base.1, z_cur) ◁ₗ uninit (PAGES (Z.to_nat remaining)))) (value (void*) (base))) ;
       (z_end @ (int (uintptr_t))) ;
       (z_cur @ (int (uintptr_t)))
-    ]
+    ]) (
+      ⌜0 ≤ given⌝ ∗
+      ⌜0 ≤ remaining⌝
+    )
   )%I.
   Typeclasses Opaque region_rec.
 
@@ -34,22 +37,25 @@ Section spec.
   Proof. solve_type_proper. Qed.
 
   Definition region : rtype := {|
-    rty_type := loc * nat * nat;
+    rty_type := loc * Z * Z;
     rty r__ := fixp region_rec r__
   |}.
 
-  Lemma region_unfold (patt__ : loc * nat * nat):
+  Lemma region_unfold (patt__ : loc * Z * Z):
     (patt__ @ region)%I ≡@{type} (
       let base := patt__.1.1 in
       let given := patt__.1.2 in
       let remaining := patt__.2 in
       let z_cur : Z := (base.2 + given * PAGE_SIZE)%Z in
       let z_end : Z := (base.2 + (given + remaining) * PAGE_SIZE)%Z in
-      struct struct_region [@{type}
-        (own_constrained (nonshr_constraint ((base.1, z_cur) ◁ₗ uninit (PAGES remaining))) (value (void*) (base))) ;
+      constrained (struct struct_region [@{type}
+        (own_constrained (nonshr_constraint ((base.1, z_cur) ◁ₗ uninit (PAGES (Z.to_nat remaining)))) (value (void*) (base))) ;
         (z_end @ (int (uintptr_t))) ;
         (z_cur @ (int (uintptr_t)))
-      ]
+      ]) (
+        ⌜0 ≤ given⌝ ∗
+        ⌜0 ≤ remaining⌝
+      )
     )%I.
   Proof. by rewrite {1}/with_refinement/=fixp_unfold. Qed.
 
@@ -78,7 +84,7 @@ Section spec.
 
   (* Specifications for function [hyp_early_alloc_nr_pages]. *)
   Definition type_of_hyp_early_alloc_nr_pages :=
-    fn(∀ (base, given, remaining) : loc * nat * nat; (global_with_type "mem" Own (((base, given, remaining)) @ (region))))
+    fn(∀ (base, given, remaining) : loc * Z * Z; (global_with_type "mem" Own (((base, given, remaining)) @ (region))))
       → ∃ () : (), (given @ (int (size_t))); (global_with_type "mem" Own (((base, given, remaining)) @ (region))).
 
   (* Specifications for function [clear_page]. *)
@@ -88,18 +94,18 @@ Section spec.
 
   (* Specifications for function [hyp_early_alloc_contig]. *)
   Definition type_of_hyp_early_alloc_contig :=
-    fn(∀ (base, given, remaining, n) : loc * nat * nat * nat; (n @ (int (u32))); (global_with_type "mem" Own (((base, given, remaining)) @ (region))) ∗ ⌜0%nat < n ≤ remaining⌝)
-      → ∃ () : (), (&own (uninit (PAGES (n)))); (global_with_type "mem" Own (((base, given + n, remaining - n)%nat) @ (region))).
+    fn(∀ (base, given, remaining, n) : loc * Z * Z * Z; (n @ (int (u32))); (global_with_type "mem" Own (((base, given, remaining)) @ (region))) ∗ ⌜0 < n ≤ remaining⌝)
+      → ∃ () : (), (&own (uninit (PAGES (Z.to_nat n)))); (global_with_type "mem" Own (((base, given + n, remaining - n)%Z) @ (region))).
 
   (* Specifications for function [hyp_early_alloc_page]. *)
   Definition type_of_hyp_early_alloc_page :=
-    fn(∀ (base, given, remaining) : loc * nat * nat; (uninit (void*)); (global_with_type "mem" Own (((base, given, remaining)) @ (region))) ∗ ⌜remaining ≠ 0%nat⌝)
-      → ∃ () : (), (&own (uninit (PAGE))); (global_with_type "mem" Own (((base, given + 1, remaining - 1)%nat) @ (region))).
+    fn(∀ (base, given, remaining) : loc * Z * Z; (uninit (void*)); (global_with_type "mem" Own (((base, given, remaining)) @ (region))) ∗ ⌜0 < remaining⌝)
+      → ∃ () : (), (&own (uninit (PAGE))); (global_with_type "mem" Own (((base, given + 1, remaining - 1)) @ (region))).
 
   (* Specifications for function [hyp_early_alloc_init]. *)
   Definition type_of_hyp_early_alloc_init :=
-    fn(∀ (l, n, s) : loc * nat * Z; (l @ (&own (uninit (PAGES (n))))), (s @ (int (u32))); ⌜s = (n * PAGE_SIZE)%Z⌝ ∗ (global_with_type "mem" Own (uninit (struct_region))))
-      → ∃ () : (), (void); (global_with_type "mem" Own (((l, 0%nat, n)) @ (region))).
+    fn(∀ (l, n, s) : loc * Z * Z; (l @ (&own (uninit (PAGES (Z.to_nat n))))), (s @ (int (u32))); ⌜s = (n * PAGE_SIZE)%Z⌝ ∗ (global_with_type "mem" Own (uninit (struct_region))))
+      → ∃ () : (), (void); (global_with_type "mem" Own (((l, 0, n)) @ (region))).
 End spec.
 
 Typeclasses Opaque region_rec.
